add new output

output/dafny_programs/05.dfy
@@ -3,75 +3,76 @@
 method IsPalindrome(s: seq<char>, i: int, j: int) returns (b: bool)
     ensures b <==> (forall k :: 0 <= k < (j - i + 1) ==> s[i + k] == s[j - k])
 {
-    var l := i;
-    var r := j;
-    while l < r
-        invariant i <= l <= r <= j
-        invariant forall k :: i <= k < l ==> s[k] == s[j - (k - i)]
-        invariant forall k :: r < k <= j ==> s[k] == s[j - (k - i)]
+    var res := true;
+    var left := i;
+    var right := j;
+    while left < right
+        invariant i <= left <= right + 1 <= j + 1 <= |s| + 1
+        invariant res ==> (forall k :: i <= k < left ==> s[k] == s[j - (k - i)])
+        decreases right - left
     {
-        if s[l] != s[r] {
-            return false;
+        if s[left] != s[right] {
+            res := false;
+            break;
         }
-        l := l + 1;
-        r := r - 1;
+        left := left + 1;
+        right := right - 1;
     }
-    return true;
+    b := res;
 }
 
-// Returns the longest palindromic substring of s
+// Main method: Returns the longest palindromic substring of s
 method LongestPalindrome(s: seq<char>) returns (res: seq<char>)
     requires |s| >= 0
     ensures (exists i, j :: 0 <= i <= j < |s| && res == s[i..j+1] && IsPalindrome(s, i, j))
-    ensures forall i, j :: 0 <= i <= j < |s| && IsPalindrome(s, i, j) ==> |s[i..j+1]| <= |res|
+    ensures (forall i, j :: 0 <= i <= j < |s| && IsPalindrome(s, i, j) ==> |res| >= j - i + 1)
 {
-    var n := |s|;
-    if n == 0 {
-        return [];
+    if |s| == 0 {
+        res := [];
+        return;
     }
-    var start := 0;
     var maxLen := 1;
+    var start := 0;
 
-    // Helper function to expand around center
-    function method Expand(s: seq<char>, left: int, right: int): int
-        requires 0 <= left < n
-        requires 0 <= right < n
-        ensures Expand(s, left, right) == (var l := left; var r := right; while l >= 0 && r < n && s[l] == s[r] { l := l - 1; r := r + 1; }; r - l - 1)
+    var i := 0;
+    while i < |s|
+        invariant 0 <= i <= |s|
+        invariant 1 <= maxLen <= |s|
+        invariant 0 <= start < |s|
+        invariant (forall k :: 0 <= k < i ==> (forall l :: 1 <= l <= maxLen ==> (exists a :: 0 <= a <= k && a + l - 1 < |s| && IsPalindrome(s, a, a + l - 1))))
+        decreases |s| - i
     {
-        var l := left;
-        var r := right;
-        while l >= 0 && r < n && s[l] == s[r] {
+        // Odd length palindrome
+        var l := i;
+        var r := i;
+        while l >= 0 && r < |s| && s[l] == s[r]
+            invariant 0 <= l + 1 <= i + 1
+            invariant i <= r < |s|
+            decreases l + 1
+        {
+            if r - l + 1 > maxLen {
+                start := l;
+                maxLen := r - l + 1;
+            }
             l := l - 1;
             r := r + 1;
         }
-        r - l - 1
-    }
-
-    var i := 0;
-    while i < n
-        invariant 0 <= i <= n
-        invariant 1 <= maxLen <= n
-        invariant 0 <= start < n
-        invariant start + maxLen <= n
-        invariant IsPalindrome(s, start, start + maxLen - 1)
-        invariant forall k :: 0 <= k < i ==> forall l, r :: 0 <= l <= r < n && IsPalindrome(s, l, r) && r - l + 1 > maxLen ==> false
-    {
-        var len1 := Expand(s, i, i);
-        var len2 := if i + 1 < n then Expand(s, i, i + 1) else 0;
-        var len := if len1 > len2 then len1 else len2;
-        if len > maxLen {
-            start := i - (len - 1) / 2;
-            maxLen := len;
+        // Even length palindrome
+        l := i;
+        r := i + 1;
+        while l >= 0 && r < |s| && s[l] == s[r]
+            invariant 0 <= l + 1 <= i + 1
+            invariant i + 1 <= r < |s| + 1
+            decreases l + 1
+        {
+            if r - l + 1 > maxLen {
+                start := l;
+                maxLen := r - l + 1;
+            }
+            l := l - 1;
+            r := r + 1;
         }
         i := i + 1;
     }
     res := s[start..start+maxLen];
-}
-
-// Example usage
-method Main()
-{
-    var s := "babad";
-    var res := LongestPalindrome(s);
-    print res, "\n";
 }
