output/dafny_programs/15.dfy
@@ -1,0 +1,80 @@
+// Dafny Specification and Program for the given Python code
+
+method ThreeSum(nums: seq<int>) returns (res: seq<seq<int>>)
+    requires true
+    ensures
+        // Each element in res is a triple of indices in nums whose sum is 0
+        forall t :: 0 <= t < |res| ==>
+            |res[t]| == 3 &&
+            res[t][0] + res[t][1] + res[t][2] == 0
+    ensures
+        // All triples in res are unique (no duplicates)
+        forall i, j :: 0 <= i < j < |res| ==> res[i] != res[j]
+    ensures
+        // All returned triples are present in nums
+        forall t :: 0 <= t < |res| ==>
+            exists i, j, k :: 
+                0 <= i < j < k < |nums| &&
+                multiset{nums[i], nums[j], nums[k]} == multiset{res[t][0], res[t][1], res[t][2]}
+{
+    var n := |nums|;
+    var arr := nums[..];
+    // Sort the array
+    var sortedNums := arr[..];
+    sortedNums := Sort(sortedNums);
+
+    if n >= 3 && sortedNums[0] == sortedNums[n - 1] && sortedNums[0] == 0 {
+        res := [ [0, 0, 0] ];
+        return;
+    }
+
+    var resultSet := set seq<int>{};
+    var resultList := new seq<seq<int>>[0];
+
+    var index := 0;
+    while index < n - 1
+        invariant 0 <= index <= n - 1
+        invariant forall t :: 0 <= t < |resultList| ==> |resultList[t]| == 3 && resultList[t][0] + resultList[t][1] + resultList[t][2] == 0
+        invariant forall i, j :: 0 <= i < j < |resultList| ==> resultList[i] != resultList[j]
+    {
+        var left := index + 1;
+        var right := n - 1;
+        while left < right
+            invariant index + 1 <= left <= right <= n - 1
+            invariant forall t :: 0 <= t < |resultList| ==> |resultList[t]| == 3 && resultList[t][0] + resultList[t][1] + resultList[t][2] == 0
+            invariant forall i, j :: 0 <= i < j < |resultList| ==> resultList[i] != resultList[j]
+        {
+            var currSum := sortedNums[index] + sortedNums[left] + sortedNums[right];
+            if currSum == 0 {
+                var triple := [sortedNums[index], sortedNums[left], sortedNums[right]];
+                if !(triple in resultSet) {
+                    resultSet := resultSet + {triple};
+                    resultList := resultList + [triple];
+                }
+                left := left + 1;
+                right := right - 1;
+            } else {
+                // In the original code, only the case currSum == 0 is handled
+                // To match the Python code, we do not move left or right otherwise
+                // So we break the loop
+                break;
+            }
+        }
+        index := index + 1;
+    }
+    res := resultList;
+}
+
+// Helper method to sort a sequence (returns a new sorted sequence)
+function method Sort(s: seq<int>): seq<int>
+    ensures multiset(s) == multiset(Sort(s))
+    ensures forall i, j :: 0 <= i < j < |Sort(s)| ==> Sort(s)[i] <= Sort(s)[j]
+{
+    if |s| <= 1 then s
+    else
+        var pivot := s[0];
+        var less := [x | x in s[1..], x < pivot];
+        var equal := [x | x in s, x == pivot];
+        var greater := [x | x in s[1..], x > pivot];
+        Sort(less) + equal + Sort(greater)
+}
